disk-betree/ImplSplit.i.dfy
@@ -7,6 +7,7 @@ module ImplSplit {
   import opened ImplCache
   import ImplModelSplit
   import opened ImplState
+  import opened ImplNode
 
   import opened Options
   import opened Maps
@@ -18,6 +19,59 @@ module ImplSplit {
   import PivotsLib
 
   import opened NativeTypes
+
+  method splitBookkeeping(k: ImplConstants, s: ImplVariables, left_childref: BT.G.Reference, right_childref: BT.G.Reference, parentref: BT.G.Reference, fused_parent_children: seq<BT.G.Reference>, left_child: Node, right_child: Node, slot: uint64)
+  requires Inv(k, s)
+  requires 0 <= slot as int < |fused_parent_children|
+  requires left_child.Inv()
+  requires right_child.Inv()
+  requires left_child.Repr !! s.Repr()
+  requires right_child.Repr !! s.Repr()
+  requires s.ready
+  modifies s.lru.Repr
+  modifies s.ephemeralIndirectionTable.Repr
+  ensures s.ready
+  ensures s.W()
+  ensures forall o | o in s.lru.Repr :: o in old(s.lru.Repr) || fresh(o)
+  ensures forall o | o in s.ephemeralIndirectionTable.Repr :: o in old(s.ephemeralIndirectionTable.Repr) || fresh(o)
+  ensures s.I() == ImplModelSplit.splitBookkeeping(Ic(k), old(s.I()), left_childref, right_childref, parentref, fused_parent_children, left_child.I(), right_child.I(), slot as int);
+  {
+    ImplModelSplit.reveal_splitBookkeeping();
+    writeBookkeeping(k, s, left_childref, left_child.children);
+    writeBookkeeping(k, s, right_childref, right_child.children);
+    writeBookkeeping(k, s, parentref, Some(replace1with2(fused_parent_children, left_childref, right_childref, slot as int)));
+  }
+
+  method splitCacheChanges(s: ImplVariables, child: Node, left_childref: BT.G.Reference,
+      right_childref: BT.G.Reference, parentref: BT.G.Reference, slot: uint64, num_children_left: uint64, pivot: Key, left_child: Node, right_child: Node)
+  requires s.ready
+  requires s.W()
+  requires s.cache.ptr(parentref).Some?
+  requires IM.WFNode(s.cache.ptr(parentref).value.I())
+  requires s.cache.ptr(parentref).value.I().children.Some?
+  requires 0 <= slot as int < |s.cache.ptr(parentref).value.I().children.value|
+  requires child.Inv()
+  requires left_child.Inv()
+  requires right_child.Inv()
+  requires left_child.Repr !! s.Repr()
+  requires right_child.Repr !! s.Repr()
+  requires left_child.Repr !! right_child.Repr
+  requires |s.cache.I()| <= 0x10000 - 2
+  requires left_childref != parentref
+  requires right_childref != parentref
+  modifies s.Repr()
+  modifies left_child.Repr // not really but it's easier to include this
+  modifies right_child.Repr
+  ensures s.W()
+  ensures (forall o | o in s.Repr() :: o in old(s.Repr()) || o in old(left_child.Repr) || o in old(right_child.Repr) || fresh(o))
+  ensures s.I() == ImplModelSplit.splitCacheChanges(old(s.I()), old(child.I()), left_childref, right_childref, parentref, slot as int, num_children_left as int, pivot, old(left_child.I()), old(right_child.I()))
+  ensures s.ready
+  {
+    ImplModelSplit.reveal_splitCacheChanges();
+    s.cache.Insert(left_childref, left_child);
+    s.cache.Insert(right_childref, right_child);
+    s.cache.SplitParent(parentref, slot as uint64, pivot, left_childref, right_childref);
+  }
 
   method doSplit(k: ImplConstants, s: ImplVariables, parentref: BT.G.Reference, ref: BT.G.Reference, slot: int)
   requires s.ready
@@ -88,17 +142,7 @@ module ImplSplit {
     var left_child := child.SplitChildLeft(num_children_left as uint64);
     var right_child := child.SplitChildRight(num_children_left as uint64);
 
-    writeBookkeeping(k, s, left_childref.value, left_child.children);
-    writeBookkeeping(k, s, right_childref.value, right_child.children);
-    writeBookkeeping(k, s, parentref, split_parent_children);
-
-    s.cache.Insert(left_childref.value, left_child);
-    s.cache.Insert(right_childref.value, right_child);
-    s.cache.SplitParent(parentref, slot as uint64, pivot, left_childref.value, right_childref.value);
-
-    assert s.W();
-    assume s.I().cache == ImplModelSplit.doSplit(Ic(k), old(s.I()), parentref, ref, slot).cache;
-    assert s.I() == ImplModelSplit.doSplit(Ic(k), old(s.I()), parentref, ref, slot);
-
+    splitBookkeeping(k, s, left_childref.value, right_childref.value, parentref, fused_parent.children.value, left_child, right_child, slot as uint64);
+    splitCacheChanges(s, child, left_childref.value, right_childref.value, parentref, slot as uint64, num_children_left as uint64, pivot, left_child, right_child);
   }
 }
